upgrade lean, draft determined

SystemFD/Metatheory/Canonicity.lean
@@ -8,10 +8,12 @@ import SystemFD.Reduction
 
 -- set_option maxHeartbeats 500000
 
+
 inductive Val : Ctx Term -> Term -> Prop where
-| app x sp : t.neutral_form = .some (x, sp)
-      -> (Γ.is_stable_red x)
-      -> Val Γ t
+| app x sp :
+  t.neutral_form = .some (x, sp) ->
+  Γ.is_stable_red x ∨ OpenVarVal Γ x sp ->
+  Val Γ t
 | choice : Val Γ t1 -> Val Γ t2 -> Val Γ (t1 ⊕ t2)
 | lam :  Val Γ (`λ[a] b)
 | lamt : Val Γ (Λ[A] b)
@@ -23,7 +25,7 @@ inductive Val : Ctx Term -> Term -> Prop where
 | eq : Val Γ (A ~[K]~ B)
 
 theorem refl_var_spine_lemma :
-  Γ.is_stable_red n ->
+  Γ.is_stable_red n ∨ OpenVarVal Γ n sp ->
   Γ ⊢ (#n).apply_spine sp : (A ~[K]~ B) ->
   False
 := by
@@ -111,47 +113,48 @@ theorem cannonical_head :
   t.neutral_form = .some (h, ts) ->
   (Γ.is_ctor h ∨ Γ.is_insttype h)
 := by
-intro vt tJ τJ tnf;
-have tshape := Term.neutral_form_law (Eq.symm tnf)
-rw[<-tshape] at tJ;
-have hJ := inversion_apply_spine tJ;
-cases hJ; case _ τ' hJ =>
-cases hJ; case _ spTy hJ =>
-cases hJ; case _ hJ h3 =>
-cases vt;
-any_goals(solve | cases tnf)
-case app h_stable tnf' =>
-  rw[tnf] at tnf'; cases tnf';
-  cases hJ; case _ wf gt =>
-  have τ'J := spine_type_is_type τJ spTy
-  have hJ := Judgment.var wf gt;
-  simp at h_stable;
-  generalize fh : Γ d@ h = f at *;
-  cases f;
-  any_goals (solve | cases gt)
-  all_goals (unfold Frame.is_stable_red at h_stable; simp at h_stable)
-  all_goals (clear h_stable; unfold Frame.get_type at gt; simp at gt; cases gt)
-  case _ =>
-    have h := ctx_get_var_type wf fh;
-    have lem1 := kind_shape h rfl
-    have lem2 := type_shape τ'J (by constructor)
-    exfalso; apply Term.is_kind_disjoint_is_type lem1 lem2
-  case _ =>
-    have h := ctx_get_datatype_kind wf fh;
-    have lem1 := kind_shape h rfl
-    have lem2 := type_shape τ'J (by constructor)
-    exfalso; apply Term.is_kind_disjoint_is_type lem1 lem2
-  case _ =>
-    apply Or.inl;
-    simp; rw[fh]; unfold Frame.is_ctor; simp;
-  case _ =>
-    have h := ctx_get_opent_kind wf fh
-    have lem1 := kind_shape h rfl
-    have lem2 := type_shape τ'J (by constructor)
-    exfalso; apply Term.is_kind_disjoint_is_type lem1 lem2
-  case _ =>
-    apply Or.inr;
-    simp; rw[fh]; unfold Frame.is_insttype; simp;
+  sorry
+-- intro vt tJ τJ tnf;
+-- have tshape := Term.neutral_form_law (Eq.symm tnf)
+-- rw[<-tshape] at tJ;
+-- have hJ := inversion_apply_spine tJ;
+-- cases hJ; case _ τ' hJ =>
+-- cases hJ; case _ spTy hJ =>
+-- cases hJ; case _ hJ h3 =>
+-- cases vt;
+-- any_goals(solve | cases tnf)
+-- case app h_stable tnf' =>
+--   rw[tnf] at tnf'; cases tnf';
+--   cases hJ; case _ wf gt =>
+--   have τ'J := spine_type_is_type τJ spTy
+--   have hJ := Judgment.var wf gt;
+--   simp at h_stable;
+--   generalize fh : Γ d@ h = f at *;
+--   cases f;
+--   any_goals (solve | cases gt)
+--   all_goals (unfold Frame.is_stable_red at h_stable; simp at h_stable)
+--   all_goals (clear h_stable; unfold Frame.get_type at gt; simp at gt; cases gt)
+--   case _ =>
+--     have h := ctx_get_var_type wf fh;
+--     have lem1 := kind_shape h rfl
+--     have lem2 := type_shape τ'J (by constructor)
+--     exfalso; apply Term.is_kind_disjoint_is_type lem1 lem2
+--   case _ =>
+--     have h := ctx_get_datatype_kind wf fh;
+--     have lem1 := kind_shape h rfl
+--     have lem2 := type_shape τ'J (by constructor)
+--     exfalso; apply Term.is_kind_disjoint_is_type lem1 lem2
+--   case _ =>
+--     apply Or.inl;
+--     simp; rw[fh]; unfold Frame.is_ctor; simp;
+--   case _ =>
+--     have h := ctx_get_opent_kind wf fh
+--     have lem1 := kind_shape h rfl
+--     have lem2 := type_shape τ'J (by constructor)
+--     exfalso; apply Term.is_kind_disjoint_is_type lem1 lem2
+--   case _ =>
+--     apply Or.inr;
+--     simp; rw[fh]; unfold Frame.is_insttype; simp;
 
 
 inductive ArrowLike : (T : Term) -> Prop where
@@ -182,192 +185,193 @@ theorem canonical_lambda :
   Judgment v Γ idx ->
   CanonicalLambdaType Γ v idx
 := by
-intro j; induction j <;> simp at *
-all_goals (intro h1 h2 h3 h4)
-any_goals try (solve | cases h1; case _ h1 => cases h1)
-any_goals try (solve | cases h3)
-case _ Γ n T wf gt ih =>
-  cases h1; case _ n_stable nnf =>
-  simp at nnf; cases nnf; case _ e1 e2 =>
-  subst e1; subst e2;
-  generalize fh : Γ d@ n = f at *;
-  unfold Frame.get_type at gt;
-  cases h4;
-  case _ =>
-    split at gt;
-    any_goals (solve | cases gt)
-    any_goals (solve | unfold Ctx.is_stable_red at n_stable; unfold Frame.is_stable_red at n_stable;
-                       exfalso; rw[fh] at n_stable; simp at n_stable)
-    all_goals (cases gt)
-    case _ =>
-      have lem := classification_lemma h3; simp at lem;
-      cases lem;
-      case _ =>
-        have wfr := @frame_wf_by_index Γ n wf;
-        have h := ctx_get_var_type wf fh;
-        cases h
-      case _ h =>
-        cases h; case _ k h => cases h; case _ _ h => cases h; case _ h => cases h
-    case _ =>
-      have wfr := @frame_wf_by_index Γ n wf;
-      have h := ctx_get_datatype_kind wf fh;
-      cases h;
-    case _ =>
-      apply LambdaLike.ctor; unfold ValidHeadVariable;
-      apply Exists.intro (n, []);
-      apply And.intro; simp; simp; rw[fh]; unfold Frame.is_ctor; simp
-    case _ =>
-      have wfr := @frame_wf_by_index Γ n wf;
-      have h := ctx_get_opent_kind wf fh;
-      cases h;
-    case _ =>
-      apply LambdaLike.insttype; unfold ValidHeadVariable;
-      apply Exists.intro (n, []);
-      apply And.intro; simp; simp; rw[fh]; unfold Frame.is_insttype; simp
-  case _ =>
-    split at gt;
-    any_goals (solve | cases gt)
-    any_goals (solve | unfold Ctx.is_stable_red at n_stable; unfold Frame.is_stable_red at n_stable;
-                       exfalso; rw[fh] at n_stable; simp at n_stable)
-    all_goals (cases gt)
-    case _ =>
-      have lem := classification_lemma h3; simp at lem;
-      cases lem;
-      case _ =>
-        have wfr := @frame_wf_by_index Γ n wf;
-        have h := ctx_get_var_type wf fh;
-        cases h
-      case _ h =>
-        cases h; case _ k h => cases h; case _ _ h => cases h; case _ h => cases h
-    case _ =>
-      have wfr := @frame_wf_by_index Γ n wf;
-      have h := ctx_get_datatype_kind wf fh;
-      cases h;
-    case _ =>
-      apply LambdaLike.ctor; unfold ValidHeadVariable;
-      apply Exists.intro (n, []);
-      apply And.intro; simp; simp; rw[fh]; unfold Frame.is_ctor; simp
-    case _ =>
-      have wfr := @frame_wf_by_index Γ n wf;
-      have h := ctx_get_opent_kind wf fh;
-      cases h;
-    case _ =>
-      apply LambdaLike.insttype; unfold ValidHeadVariable;
-      apply Exists.intro (n, []);
-      apply And.intro; simp; simp; rw[fh]; unfold Frame.is_insttype; simp
+  sorry
+-- intro j; induction j <;> simp at *
+-- all_goals (intro h1 h2 h3 h4)
+-- any_goals try (solve | cases h1; case _ h1 => cases h1)
+-- any_goals try (solve | cases h3)
+-- case _ Γ n T wf gt ih =>
+--   cases h1; case _ n_stable nnf =>
+--   simp at nnf; cases nnf; case _ e1 e2 =>
+--   subst e1; subst e2;
+--   generalize fh : Γ d@ n = f at *;
+--   unfold Frame.get_type at gt;
+--   cases h4;
+--   case _ =>
+--     split at gt;
+--     any_goals (solve | cases gt)
+--     any_goals (solve | unfold Ctx.is_stable_red at n_stable; unfold Frame.is_stable_red at n_stable;
+--                        exfalso; rw[fh] at n_stable; simp at n_stable)
+--     all_goals (cases gt)
+--     case _ =>
+--       have lem := classification_lemma h3; simp at lem;
+--       cases lem;
+--       case _ =>
+--         have wfr := @frame_wf_by_index Γ n wf;
+--         have h := ctx_get_var_type wf fh;
+--         cases h
+--       case _ h =>
+--         cases h; case _ k h => cases h; case _ _ h => cases h; case _ h => cases h
+--     case _ =>
+--       have wfr := @frame_wf_by_index Γ n wf;
+--       have h := ctx_get_datatype_kind wf fh;
+--       cases h;
+--     case _ =>
+--       apply LambdaLike.ctor; unfold ValidHeadVariable;
+--       apply Exists.intro (n, []);
+--       apply And.intro; simp; simp; rw[fh]; unfold Frame.is_ctor; simp
+--     case _ =>
+--       have wfr := @frame_wf_by_index Γ n wf;
+--       have h := ctx_get_opent_kind wf fh;
+--       cases h;
+--     case _ =>
+--       apply LambdaLike.insttype; unfold ValidHeadVariable;
+--       apply Exists.intro (n, []);
+--       apply And.intro; simp; simp; rw[fh]; unfold Frame.is_insttype; simp
+--   case _ =>
+--     split at gt;
+--     any_goals (solve | cases gt)
+--     any_goals (solve | unfold Ctx.is_stable_red at n_stable; unfold Frame.is_stable_red at n_stable;
+--                        exfalso; rw[fh] at n_stable; simp at n_stable)
+--     all_goals (cases gt)
+--     case _ =>
+--       have lem := classification_lemma h3; simp at lem;
+--       cases lem;
+--       case _ =>
+--         have wfr := @frame_wf_by_index Γ n wf;
+--         have h := ctx_get_var_type wf fh;
+--         cases h
+--       case _ h =>
+--         cases h; case _ k h => cases h; case _ _ h => cases h; case _ h => cases h
+--     case _ =>
+--       have wfr := @frame_wf_by_index Γ n wf;
+--       have h := ctx_get_datatype_kind wf fh;
+--       cases h;
+--     case _ =>
+--       apply LambdaLike.ctor; unfold ValidHeadVariable;
+--       apply Exists.intro (n, []);
+--       apply And.intro; simp; simp; rw[fh]; unfold Frame.is_ctor; simp
+--     case _ =>
+--       have wfr := @frame_wf_by_index Γ n wf;
+--       have h := ctx_get_opent_kind wf fh;
+--       cases h;
+--     case _ =>
+--       apply LambdaLike.insttype; unfold ValidHeadVariable;
+--       apply Exists.intro (n, []);
+--       apply And.intro; simp; simp; rw[fh]; unfold Frame.is_insttype; simp
 
-case _ Γ f _ _ _ fJ _ _ ih => -- appk bogus case
-  cases h1; case _ n ts n_stable ts' =>
-  simp at ts'; rw [Option.bind_eq_some] at ts';  cases ts'; case _ w fnf =>
-  cases fnf; case _ fnf ts' =>
-  cases ts';
-  have vf : Val Γ f := by constructor; assumption; assumption
-  generalize fh : Γ d@ w.fst = f at *;
-  have lem := classification_lemma fJ; simp at lem; cases lem;
-  case _ h => cases h; case _ k1 k2 =>
-    have lem1 := kind_shape k2 rfl
-    have lem2 := type_shape h3 (by constructor)
-    exfalso; apply Term.is_kind_disjoint_is_type lem1 lem2
-  case _ h =>
-    cases h; case _ w h =>
-    cases h; case _ wk arrk =>
-    cases arrk; cases wk;
+-- case _ Γ f _ _ _ fJ _ _ ih => -- appk bogus case
+--   cases h1; case _ n ts n_stable ts' =>
+--   simp at ts'; rw [Option.bind_eq_some] at ts';  cases ts'; case _ w fnf =>
+--   cases fnf; case _ fnf ts' =>
+--   cases ts';
+--   have vf : Val Γ f := by constructor; assumption; assumption
+--   generalize fh : Γ d@ w.fst = f at *;
+--   have lem := classification_lemma fJ; simp at lem; cases lem;
+--   case _ h => cases h; case _ k1 k2 =>
+--     have lem1 := kind_shape k2 rfl
+--     have lem2 := type_shape h3 (by constructor)
+--     exfalso; apply Term.is_kind_disjoint_is_type lem1 lem2
+--   case _ h =>
+--     cases h; case _ w h =>
+--     cases h; case _ wk arrk =>
+--     cases arrk; cases wk;
 
-case lam Γ A t B ih1 ih2 => constructor
+-- case lam Γ A t B ih1 ih2 => constructor
 
-case app Γ f A B a B' fJ aJ h0 ih1 ih2 =>
-  cases h1; case _ n ts n_stable h1 =>
-  simp at h1; rw[Option.bind_eq_some] at h1;
-  cases h1;  case _ ts' fnf =>
-  cases fnf; case _ fnf hts =>
-  cases ts'; case _ x sp =>
-  simp at hts; cases hts; case _ e1 e2 =>
-  subst e1; subst e2
-  have h := Val.app x sp fnf n_stable;
-  simp at *;
-  have lem := classification_lemma fJ; simp at lem;
-  cases lem;
-  case _ h => cases h
-  case _ h =>
-    cases h; case _ k h =>
-    cases h; case _ k h =>
-    cases h; case _ aK bK =>
-    have arrK := Judgment.arrow aK bK;
-    have ih := ih1 h fJ arrK (ArrowLike.arrowt); cases ih;
-    case _ h => cases fnf
-    case _ h => cases fnf
-    case _ h =>
-      apply LambdaLike.ctor;
-      unfold ValidHeadVariable;
-      have fanf := @Term.neutral_form_app f a x sp fnf; symm at fanf;
-      apply Exists.intro (x, sp ++ [(.term, a)]);
-      apply And.intro; assumption; simp;
-      unfold ValidHeadVariable at h; simp at h;
-      cases h; case _ h => cases h; case _ fnf' h =>
-      rw [fnf] at fnf'; cases fnf'; case _ h =>
-      cases h; assumption
-    case _ h =>
-      apply LambdaLike.insttype;
-      unfold ValidHeadVariable;
-      have fanf := @Term.neutral_form_app f a x sp fnf; symm at fanf;
-      apply Exists.intro (x, sp ++ [(.term, a)]);
-      apply And.intro; assumption; simp;
-      unfold ValidHeadVariable at h; simp at h;
-      cases h; case _ h => cases h; case _ fnf' h =>
-      rw [fnf] at fnf'; cases fnf'; case _ h =>
-      cases h; assumption
-    case _ => cases fnf
-case _ ih1 _ =>
-  cases h1;
-  case _ h => cases h
-  case _ => constructor
+-- case app Γ f A B a B' fJ aJ h0 ih1 ih2 =>
+--   cases h1; case _ n ts n_stable h1 =>
+--   simp at h1; rw[Option.bind_eq_some] at h1;
+--   cases h1;  case _ ts' fnf =>
+--   cases fnf; case _ fnf hts =>
+--   cases ts'; case _ x sp =>
+--   simp at hts; cases hts; case _ e1 e2 =>
+--   subst e1; subst e2
+--   have h := Val.app x sp fnf n_stable;
+--   simp at *;
+--   have lem := classification_lemma fJ; simp at lem;
+--   cases lem;
+--   case _ h => cases h
+--   case _ h =>
+--     cases h; case _ k h =>
+--     cases h; case _ k h =>
+--     cases h; case _ aK bK =>
+--     have arrK := Judgment.arrow aK bK;
+--     have ih := ih1 h fJ arrK (ArrowLike.arrowt); cases ih;
+--     case _ h => cases fnf
+--     case _ h => cases fnf
+--     case _ h =>
+--       apply LambdaLike.ctor;
+--       unfold ValidHeadVariable;
+--       have fanf := @Term.neutral_form_app f a x sp fnf; symm at fanf;
+--       apply Exists.intro (x, sp ++ [(.term, a)]);
+--       apply And.intro; assumption; simp;
+--       unfold ValidHeadVariable at h; simp at h;
+--       cases h; case _ h => cases h; case _ fnf' h =>
+--       rw [fnf] at fnf'; cases fnf'; case _ h =>
+--       cases h; assumption
+--     case _ h =>
+--       apply LambdaLike.insttype;
+--       unfold ValidHeadVariable;
+--       have fanf := @Term.neutral_form_app f a x sp fnf; symm at fanf;
+--       apply Exists.intro (x, sp ++ [(.term, a)]);
+--       apply And.intro; assumption; simp;
+--       unfold ValidHeadVariable at h; simp at h;
+--       cases h; case _ h => cases h; case _ fnf' h =>
+--       rw [fnf] at fnf'; cases fnf'; case _ h =>
+--       cases h; assumption
+--     case _ => cases fnf
+-- case _ ih1 _ =>
+--   cases h1;
+--   case _ h => cases h
+--   case _ => constructor
 
-case _ Γ f A B a B' fJ aJ _ ih1 ih2 =>
-  cases h1; case _ n ts n_stable h1 =>
-  simp at h1; rw[Option.bind_eq_some] at h1;
-  cases h1;  case _ ts' fnf =>
-  cases fnf; case _ fnf hts =>
-  cases ts'; case _ x sp =>
-  simp at hts; cases hts; case _ e1 e2 =>
-  subst e1; subst e2
-  have h := Val.app x sp fnf n_stable;
-  simp at *;
-  have lem := classification_lemma fJ; simp at lem;
-  cases lem;
-  case _ h => cases h
-  case _ h =>
-    cases h; case _ k h =>
-    cases h; case _ k h =>
-    cases h; case _ aK bK =>
-    have arrK := Judgment.allt aK bK;
-    have ih := ih1 h fJ arrK (ArrowLike.allt); cases ih;
-    case _ h => cases fnf
-    case _ h => cases fnf
-    case _ h =>
-        apply LambdaLike.ctor;
-        unfold ValidHeadVariable;
-        have fanf := @Term.neutral_form_appt f a x sp fnf; symm at fanf;
-        apply Exists.intro (x, sp ++ [(.type, a)]);
-        apply And.intro; assumption; simp;
-        unfold ValidHeadVariable at h; simp at h;
-        cases h; case _ h => cases h; case _ fnf' h =>
-        rw [fnf] at fnf'; cases fnf'; case _ h =>
-        cases h; assumption;
-    case _ h =>
-        apply LambdaLike.insttype;
-        unfold ValidHeadVariable;
-        have fanf := @Term.neutral_form_appt f a x sp fnf; symm at fanf;
-        apply Exists.intro (x, sp ++ [(.type, a)]);
-        apply And.intro; assumption; simp;
-        unfold ValidHeadVariable at h; simp at h;
-        cases h; case _ h => cases h; case _ fnf' h =>
-        rw [fnf] at fnf'; cases fnf'; case _ h =>
-        cases h; assumption;
-    case _ => cases fnf
-case _ ih2 => cases h4
-case choice j1 j2 j3 j4 ih1 ih2 ih3 ih4 =>
-  cases h1; case _ h => cases h
-  case _ v1 v2 =>
-    replace ih3 := ih3 v1 j3 h3 h4
-    replace ih4 := ih4 v2 j4 h3 h4
-    apply LambdaLike.choice ih3 ih4
+-- case _ Γ f A B a B' fJ aJ _ ih1 ih2 =>
+--   cases h1; case _ n ts n_stable h1 =>
+--   simp at h1; rw[Option.bind_eq_some] at h1;
+--   cases h1;  case _ ts' fnf =>
+--   cases fnf; case _ fnf hts =>
+--   cases ts'; case _ x sp =>
+--   simp at hts; cases hts; case _ e1 e2 =>
+--   subst e1; subst e2
+--   have h := Val.app x sp fnf n_stable;
+--   simp at *;
+--   have lem := classification_lemma fJ; simp at lem;
+--   cases lem;
+--   case _ h => cases h
+--   case _ h =>
+--     cases h; case _ k h =>
+--     cases h; case _ k h =>
+--     cases h; case _ aK bK =>
+--     have arrK := Judgment.allt aK bK;
+--     have ih := ih1 h fJ arrK (ArrowLike.allt); cases ih;
+--     case _ h => cases fnf
+--     case _ h => cases fnf
+--     case _ h =>
+--         apply LambdaLike.ctor;
+--         unfold ValidHeadVariable;
+--         have fanf := @Term.neutral_form_appt f a x sp fnf; symm at fanf;
+--         apply Exists.intro (x, sp ++ [(.type, a)]);
+--         apply And.intro; assumption; simp;
+--         unfold ValidHeadVariable at h; simp at h;
+--         cases h; case _ h => cases h; case _ fnf' h =>
+--         rw [fnf] at fnf'; cases fnf'; case _ h =>
+--         cases h; assumption;
+--     case _ h =>
+--         apply LambdaLike.insttype;
+--         unfold ValidHeadVariable;
+--         have fanf := @Term.neutral_form_appt f a x sp fnf; symm at fanf;
+--         apply Exists.intro (x, sp ++ [(.type, a)]);
+--         apply And.intro; assumption; simp;
+--         unfold ValidHeadVariable at h; simp at h;
+--         cases h; case _ h => cases h; case _ fnf' h =>
+--         rw [fnf] at fnf'; cases fnf'; case _ h =>
+--         cases h; assumption;
+--     case _ => cases fnf
+-- case _ ih2 => cases h4
+-- case choice j1 j2 j3 j4 ih1 ih2 ih3 ih4 =>
+--   cases h1; case _ h => cases h
+--   case _ v1 v2 =>
+--     replace ih3 := ih3 v1 j3 h3 h4
+--     replace ih4 := ih4 v2 j4 h3 h4
+--     apply LambdaLike.choice ih3 ih4
