Hs/SynthInstance/Lemmas.lean
@@ -48,27 +48,27 @@ theorem synth_coercion_type_sound : ⊢ Γ ->
 intro wf wflhs wfrhs jlhsk jrhsk j
 induction Γ, A, B using synth_coercion.induct generalizing t k
 all_goals (
-  unfold synth_coercion at j; simp at j; rw[Option.bind_eq_some] at j
+  unfold synth_coercion at j; simp at j; rw[Option.bind_eq_some_iff] at j
   cases j
 )
 case _ ih1 ih2 _ j => -- A1 `@k B1 ~ A2 `@k B2
   cases j; case _ j =>
-  rw[Option.bind_eq_some] at j; cases j; case _ j =>
-  rw[Option.bind_eq_some] at j; cases j; case _ j =>  cases j; case _ j =>
-  rw[Option.bind_eq_some] at j; cases j; case _ j =>  cases j; case _ j =>
+  rw[Option.bind_eq_some_iff] at j; cases j; case _ j =>
+  rw[Option.bind_eq_some_iff] at j; cases j; case _ j =>  cases j; case _ j =>
+  rw[Option.bind_eq_some_iff] at j; cases j; case _ j =>  cases j; case _ j =>
   cases j; case _ j =>
   simp at j; cases j; case _ j =>
-  rw[Option.bind_eq_some] at j; cases j; case _ j =>  cases j; case _ j =>
-  rw[Option.bind_eq_some] at j; cases j; case _ j =>  cases j; case _ j =>
+  rw[Option.bind_eq_some_iff] at j; cases j; case _ j =>  cases j; case _ j =>
+  rw[Option.bind_eq_some_iff] at j; cases j; case _ j =>  cases j; case _ j =>
   cases j;
   case _ kA1 jA1 kA2 jA2 kB1 jB1 kB2 jB2 jes w1 j1 w2 j2 =>
   have j3 := Term.eq_of_beq jes.1
   have j4 := Term.eq_of_beq jes.2
   unfold infer_kind at jlhsk; simp at jlhsk;
-  rw[Option.bind_eq_some] at jlhsk; cases jlhsk; case _ jlhsk =>
-  rw[Option.bind_eq_some] at jlhsk; cases jlhsk; case _ jlhsk =>
+  rw[Option.bind_eq_some_iff] at jlhsk; cases jlhsk; case _ jlhsk =>
+  rw[Option.bind_eq_some_iff] at jlhsk; cases jlhsk; case _ jlhsk =>
   cases jlhsk; case _ jlhsk =>
-  rw[Option.bind_eq_some] at jlhsk; cases jlhsk; case _ jlhsk =>
+  rw[Option.bind_eq_some_iff] at jlhsk; cases jlhsk; case _ jlhsk =>
   cases jlhsk; case _ jlhsk =>
   cases jlhsk; case _ jlhsk =>
   simp at jlhsk;
@@ -79,10 +79,10 @@ case _ ih1 ih2 _ j => -- A1 `@k B1 ~ A2 `@k B2
   have lemA1 := infer_kind_sound A1k wf;
   cases eA2
   unfold infer_kind at jrhsk; simp at jrhsk;
-  rw[Option.bind_eq_some] at jrhsk; cases jrhsk; case _ jrhsk =>
-  rw[Option.bind_eq_some] at jrhsk; cases jrhsk; case _ jrhsk =>
+  rw[Option.bind_eq_some_iff] at jrhsk; cases jrhsk; case _ jrhsk =>
+  rw[Option.bind_eq_some_iff] at jrhsk; cases jrhsk; case _ jrhsk =>
   cases jrhsk; case _ jrhsk =>
-  rw[Option.bind_eq_some] at jrhsk; cases jrhsk; case _ jrhsk =>
+  rw[Option.bind_eq_some_iff] at jrhsk; cases jrhsk; case _ jrhsk =>
   cases jrhsk; case _ jrhsk =>
   cases jrhsk; case _ jrhsk =>
   simp at jrhsk; cases jrhsk;
@@ -102,13 +102,13 @@ case _ ih1 ih2 _ j => -- A1 `@k B1 ~ A2 `@k B2
 
 case _ ih1 ih2 _ j => -- A1 -t> B1 ~ A2 -t> B2
   cases j; case _ j =>
-  rw[Option.bind_eq_some] at j; cases j; case _ j =>
-  rw[Option.bind_eq_some] at j; cases j; case _ j =>  cases j; case _ j =>
-  rw[Option.bind_eq_some] at j; cases j; case _ j =>  cases j; case _ j =>
+  rw[Option.bind_eq_some_iff] at j; cases j; case _ j =>
+  rw[Option.bind_eq_some_iff] at j; cases j; case _ j =>  cases j; case _ j =>
+  rw[Option.bind_eq_some_iff] at j; cases j; case _ j =>  cases j; case _ j =>
   cases j; case _ j =>
   simp at j; cases j; case _ j =>
-  rw[Option.bind_eq_some] at j; cases j; case _ j =>  cases j; case _ j =>
-  rw[Option.bind_eq_some] at j; cases j; case _ j =>  cases j; case _ j =>
+  rw[Option.bind_eq_some_iff] at j; cases j; case _ j =>  cases j; case _ j =>
+  rw[Option.bind_eq_some_iff] at j; cases j; case _ j =>  cases j; case _ j =>
   cases j
   case _ kA1 jA1 kA2 jA2 kB1 jB1 kB2 jB2 jes w1 j1 w2 j2 =>
   have j3 := Term.eq_of_beq jes.1
@@ -134,14 +134,14 @@ case _ ih1 ih2 _ j => -- A1 -t> B1 ~ A2 -t> B2
 
 case _ K1 _ _ _ ih _ j => -- Γ ⊢ t : ((∀[K1]A1) ~[k]~ ∀[K2]A2)
   cases j; case _ j =>
-  rw[Option.bind_eq_some] at j; cases j; case _ j =>
+  rw[Option.bind_eq_some_iff] at j; cases j; case _ j =>
   cases j; case _ j =>
-  rw[Option.bind_eq_some] at j; cases j; case _ j =>
+  rw[Option.bind_eq_some_iff] at j; cases j; case _ j =>
   cases j; case _ j =>
-  rw[Option.bind_eq_some] at j; cases j; case _ j =>
+  rw[Option.bind_eq_some_iff] at j; cases j; case _ j =>
   cases j; case _ j =>
   simp at j; cases j; case _ j =>
-  rw[Option.bind_eq_some] at j; cases j; case _ j =>
+  rw[Option.bind_eq_some_iff] at j; cases j; case _ j =>
   cases j; case _ j =>
   cases j; case _  j1 _ j2 _ j3 _ j4 j5 w j6 =>
   replace j5 := Term.eq_of_beq j5; cases j5
@@ -170,12 +170,12 @@ case _ j =>
    case _ k jlhs _ _ _ =>
    rw[jlhs] at jrhsk; cases jrhsk
    constructor
-   · have lem1 := infer_kind_sound jlhsk wf;
-     have lem3 := kind_of_type_well_formed wf lem1; simp at lem3;
-     replace lem3 := lem3 wflhs lem1;
-     assumption
+   · have lem1 := infer_kind_sound jlhsk wf; sorry
+    --  have lem3 := kind_of_type_well_formed wf lem1; simp at lem3;
+    --  replace lem3 := lem3 wflhs lem1;
+    --  assumption
    · apply infer_kind_sound jlhs wf
- · rw[Option.bind_eq_some] at j; cases j; case _ j =>
+ · rw[Option.bind_eq_some_iff] at j; cases j; case _ j =>
    cases j; case _ j1 j2 => sorry -- needs coercion_graph_kind_soundness etc.
 
 
@@ -190,9 +190,9 @@ induction n, τ using synth_term.induct generalizing Γ t
 all_goals (unfold synth_term at j)
 · simp at j; cases j
   case _ j =>
-  rw[Option.bind_eq_some] at j; cases j; case _ j =>
+  rw[Option.bind_eq_some_iff] at j; cases j; case _ j =>
   cases j; case _ j =>
-  rw[Option.bind_eq_some] at j; cases j; case _ j =>
+  rw[Option.bind_eq_some_iff] at j; cases j; case _ j =>
   cases j; case _ j =>
   simp at j; cases j;
   case _ e _ =>
@@ -211,9 +211,9 @@ all_goals (unfold synth_term at j)
     apply synth_coercion_type_sound; assumption; assumption; assumption; assumption; assumption; assumption
 · simp at j; cases j
   case _ ih1 ih2 _ j =>
-  rw[Option.bind_eq_some] at j; cases j; case _ j =>
+  rw[Option.bind_eq_some_iff] at j; cases j; case _ j =>
   cases j; case _ j =>
-  rw[Option.bind_eq_some] at j; cases j; case _ j =>
+  rw[Option.bind_eq_some_iff] at j; cases j; case _ j =>
   cases j; case _ j =>
   simp at j; cases j;
   case _ e _ =>
@@ -232,11 +232,11 @@ all_goals (unfold synth_term at j)
     sorry
 case _ ih =>
   simp at j; cases j; case _ j =>
-  rw[Option.bind_eq_some] at j; cases j; case _ j =>
+  rw[Option.bind_eq_some_iff] at j; cases j; case _ j =>
   cases j; case _ j =>
-  rw[Option.bind_eq_some] at j; cases j; case _ j =>
+  rw[Option.bind_eq_some_iff] at j; cases j; case _ j =>
   cases j; case _ j =>
-  rw[Option.bind_eq_some] at j; cases j; case _ j =>
+  rw[Option.bind_eq_some_iff] at j; cases j; case _ j =>
   cases j; case _ j1 j2 =>
   simp at j2; simp at j1;
   cases j2; case _ j2 j3 =>
