Hs/Translator/Lemmas/TypesSoundness.lean
@@ -88,7 +88,7 @@ case _ =>
 
   simp at ls; cases ls;
   case _ =>
-    rw[Option.bind_eq_some] at h1; cases h1; case _ w h1 =>
+    rw[Option.bind_eq_some_iff] at h1; cases h1; case _ w h1 =>
     cases h1; case _ h1 e =>
     simp at e; cases e; case _ e1 e2 =>
     have e := @Prod.mk.eta (List Term) Term w
@@ -117,7 +117,7 @@ case _ τ τs ih =>
       apply lem2 k; simp_all
     assumption
   case _ =>
-    rw[Option.bind_eq_some] at h1; cases h1; case _ w h1 =>
+    rw[Option.bind_eq_some_iff] at h1; cases h1; case _ w h1 =>
     cases h1; case _ w1 h1 =>
     injection h1; case _ h1 =>
     injection h1; case _ h1a h1b =>
@@ -170,95 +170,96 @@ theorem compile_type_shape_soundness (Γ : Ctx Term) (k : Term) (τ : HsTerm) (�
  Term.IsKind k ->
  compile_type Γ k τ = .ok τ' ->
  Term.IsType τ' := by
-intro wf j1 j2 j3
-induction Γ, k, τ using compile_type.induct generalizing τ' <;> simp at *
+sorry
+-- intro wf j1 j2 j3
+-- induction Γ, k, τ using compile_type.induct generalizing τ' <;> simp at *
 
-all_goals try (
-case _ ih1 ih2 =>
-  cases j3; case _ j3 =>
-  cases j3; case _ j3 =>
-  cases j3; cases j1; case _ h1 _ h2 h3 h4 =>
-  cases h2; case _ A' B' h2 e =>
-  cases e
-  have ih1' := ih1 A' wf h3 (by constructor) h1
-  replace ih2 := ih2 B' (Judgment.wfempty wf) h4 (by constructor) h2
-  constructor; assumption; assumption)
+-- all_goals try (
+-- case _ ih1 ih2 =>
+--   cases j3; case _ j3 =>
+--   cases j3; case _ j3 =>
+--   cases j3; cases j1; case _ h1 _ h2 h3 h4 =>
+--   cases h2; case _ A' B' h2 e =>
+--   cases e
+--   have ih1' := ih1 A' wf h3 (by constructor) h1
+--   replace ih2 := ih2 B' (Judgment.wfempty wf) h4 (by constructor) h2
+--   constructor; assumption; assumption)
 
-case _ Γ K A ih =>
-  cases j3; case _ j3 =>
-  cases j3; case _ j3 =>
-  cases j3; cases j1; case _ K' h1 A' h2 h3 h4 =>
-  cases h2; case _ h2 e =>
-  cases e
-  have lem' : Except.ok K' = DsM.ok K' := by simp
-  rw[lem'] at h1;
+-- case _ Γ K A ih =>
+--   cases j3; case _ j3 =>
+--   cases j3; case _ j3 =>
+--   cases j3; cases j1; case _ K' h1 A' h2 h3 h4 =>
+--   cases h2; case _ h2 e =>
+--   cases e
+--   have lem' : Except.ok K' = DsM.ok K' := by simp
+--   rw[lem'] at h1;
 
-  have lem := compile_kind_sound wf h3 h1
-  have wf' : ⊢ (.kind K' :: Γ) := by constructor; assumption; assumption
-  replace ih := @ih K' A' wf' h4 (by constructor) h2
-  have lem := kind_shape lem rfl
-  constructor; assumption; assumption
+--   have lem := compile_kind_sound wf h3 h1
+--   have wf' : ⊢ (.kind K' :: Γ) := by constructor; assumption; assumption
+--   replace ih := @ih K' A' wf' h4 (by constructor) h2
+--   have lem := kind_shape lem rfl
+--   constructor; assumption; assumption
 
-case _ tnf _ _ _ => simp_all; rw[tnf] at j3; simp at j3
-case _ sp idx _ tnfp _ _ _ _ =>
- split at j3
- case _ => cases j3
- case _ =>
- split at j3
- /- head is a variable -/
- case _ =>
-   simp at j3; cases j3; case _ n tnfp idx tnfp' κ j3 =>
-   rw[tnfp] at tnfp'; cases tnfp'
-   case _ tnfp' tnfp'' _ _ _ _ _ =>
-   rw[tnfp] at tnfp'; cases tnfp'; clear tnfp''; cases j3; case _ j4 j3 =>
-   simp at j3; split at j3
-   case _ wfk =>
-     split at j3
-     case _ => simp at j3
-     case _ κs ret_κ h1 =>
-     split at j3
-     case _ j4 =>
-       simp at j4
-       cases j4; case _ j4 j5 =>
-       cases j4; case _ j4 j6 =>
-       have e := Term.eq_of_beq j4; cases e; clear j4
-       rw[Except.bind_eq_ok] at j3; cases j3
-       case _ exp_κ τ _ _ _ ih τs j3 =>
-       cases j3; case _ j3 j7 =>
-       cases j7; rw[List.foldl_eq_foldr_reverse]
-       have lem1 := HsTerm.hs_type_neutral_form_is_type j1 tnfp
-       have lem2 := HsTerm.hs_is_type_neutral_form j1 tnfp -- TODO Use Lem1 here
-       rw[<-List.mapM'_eq_mapM] at j3
+-- case _ tnf _ _ _ => simp_all; rw[tnf] at j3; simp at j3
+-- case _ sp idx _ tnfp _ _ _ _ =>
+--  split at j3
+--  case _ => cases j3
+--  case _ =>
+--  split at j3
+--  /- head is a variable -/
+--  case _ =>
+--    simp at j3; cases j3; case _ n tnfp idx tnfp' κ j3 =>
+--    rw[tnfp] at tnfp'; cases tnfp'
+--    case _ tnfp' tnfp'' _ _ _ _ _ =>
+--    rw[tnfp] at tnfp'; cases tnfp'; clear tnfp''; cases j3; case _ j4 j3 =>
+--    simp at j3; split at j3
+--    case _ wfk =>
+--      split at j3
+--      case _ => simp at j3
+--      case _ κs ret_κ h1 =>
+--      split at j3
+--      case _ j4 =>
+--        simp at j4
+--        cases j4; case _ j4 j5 =>
+--        cases j4; case _ j4 j6 =>
+--        have e := Term.eq_of_beq j4; cases e; clear j4
+--        rw[Except.bind_eq_ok] at j3; cases j3
+--        case _ exp_κ τ _ _ _ ih τs j3 =>
+--        cases j3; case _ j3 j7 =>
+--        cases j7; rw[List.foldl_eq_foldr_reverse]
+--        have lem1 := HsTerm.hs_type_neutral_form_is_type j1 tnfp
+--        have lem2 := HsTerm.hs_is_type_neutral_form j1 tnfp -- TODO Use Lem1 here
+--        rw[<-List.mapM'_eq_mapM] at j3
 
-       cases lem1; case _ lem1a =>
-       have κ_wf : κ.IsKind := wf_kind_shape_sound wfk
-       have lem3 := kind_shape_split_arrow κ_wf h1
-       cases lem3; case _ lem3a lem3b =>
-       apply is_type_spine_application
-       case _ => constructor
-       case _ ih _ _ =>
-         intro τ' τ'_in_τs
-         have lem3 := mapM'_elems_image j3 τ' τ'_in_τs
-         cases lem3; case _ lem3 =>
-         cases lem3; case _ w w_in_sp lem3 =>
-         simp at lem3; split at lem3 <;> simp at lem3
-         case _ contra => simp at contra
-         case _ e _ =>
-           have lem2' := lem2 (w.val.snd.val.fst, w.val.snd.val.snd) w.val.snd.property
-           simp at lem2'; cases lem2'
-           apply ih κs w.val.fst w.val.fst.property (w.val.snd.val.fst) _ _ _ τ' wf _ _ lem3
-           apply w.val.snd.property
-           apply w.property
-           assumption
-           apply lem3b w.val.fst.val w.val.fst.property
-         case _ contra => simp at contra
+--        cases lem1; case _ lem1a =>
+--        have κ_wf : κ.IsKind := wf_kind_shape_sound wfk
+--        have lem3 := kind_shape_split_arrow κ_wf h1
+--        cases lem3; case _ lem3a lem3b =>
+--        apply is_type_spine_application
+--        case _ => constructor
+--        case _ ih _ _ =>
+--          intro τ' τ'_in_τs
+--          have lem3 := mapM'_elems_image j3 τ' τ'_in_τs
+--          cases lem3; case _ lem3 =>
+--          cases lem3; case _ w w_in_sp lem3 =>
+--          simp at lem3; split at lem3 <;> simp at lem3
+--          case _ contra => simp at contra
+--          case _ e _ =>
+--            have lem2' := lem2 (w.val.snd.val.fst, w.val.snd.val.snd) w.val.snd.property
+--            simp at lem2'; cases lem2'
+--            apply ih κs w.val.fst w.val.fst.property (w.val.snd.val.fst) _ _ _ τ' wf _ _ lem3
+--            apply w.val.snd.property
+--            apply w.property
+--            assumption
+--            apply lem3b w.val.fst.val w.val.fst.property
+--          case _ contra => simp at contra
 
-     case _ => simp at j3
-   case _ => simp at j3
+--      case _ => simp at j3
+--    case _ => simp at j3
 
- /- head is a not a variable, bogus case -/
- case _ => cases j3
-case _ tnf _ _ _ _ => simp_all; rw[tnf] at j3; simp at j3;
+--  /- head is a not a variable, bogus case -/
+--  case _ => cases j3
+-- case _ tnf _ _ _ _ => simp_all; rw[tnf] at j3; simp at j3;
 
 -- theorem compile_type_sound (k : Term) (τ : HsTerm) :
 --   ⊢ Γ ->
@@ -398,7 +399,7 @@ intro j
 induction j generalizing h sp <;> simp at *
 case _ ih1 ih2 =>
  intro h1;
- rw[Option.bind_eq_some] at h1
+ rw[Option.bind_eq_some_iff] at h1
  cases h1; case _ w h1 =>
  cases h1; case _ h1a h2a =>
  injection h2a; case _ h2a =>
@@ -476,7 +477,7 @@ theorem type_heads_varty : ⊢s Γ ->
 intro wf j; induction j <;> simp at *
 case _ j _ ih _ _ =>
 intro x sp j' tnf
-rw[Option.bind_eq_some] at tnf; cases tnf; case _ w tnf =>
+rw[Option.bind_eq_some_iff] at tnf; cases tnf; case _ w tnf =>
 cases tnf; case _ h1 h2 =>
 injection h2; case _ h2 =>
 injection h2; case _ h2 h3 =>
@@ -519,121 +520,122 @@ theorem compile_type_soundness :
   CtxEquiv Γ Γ' ->
   HsJudgment i Γ jty ->
   CompileTypeSoundnessLemmaType Γ' i jty := by
-intro wf Γe j
-induction j generalizing Γ' <;> simp at *
+sorry
+-- intro wf Γe j
+-- induction j generalizing Γ' <;> simp at *
 
-case _ ih1 ih2 => -- arrow
-  replace ih1 := @ih1 Γ' wf Γe
-  cases ih1; case _ A' ih1 =>
-  cases ih1; case _ ih1 =>
+-- case _ ih1 ih2 => -- arrow
+--   replace ih1 := @ih1 Γ' wf Γe
+--   cases ih1; case _ A' ih1 =>
+--   cases ih1; case _ ih1 =>
 
-  replace ih2 := @ih2 (.empty :: Γ') (by constructor; assumption) (by apply lift_ctx_equiv; assumption)
+--   replace ih2 := @ih2 (.empty :: Γ') (by constructor; assumption) (by apply lift_ctx_equiv; assumption)
 
-  cases ih2; case _ B' ih2 =>
-  cases ih2; case _ ih2 =>
-  exists (A' -t> B')
-  constructor
-  exists A';
-  constructor;
-  case _ => assumption
-  case _ => exists B';
-  constructor; assumption; assumption
+--   cases ih2; case _ B' ih2 =>
+--   cases ih2; case _ ih2 =>
+--   exists (A' -t> B')
+--   constructor
+--   exists A';
+--   constructor;
+--   case _ => assumption
+--   case _ => exists B';
+--   constructor; assumption; assumption
 
-case _ j1 j2 j3 _ _ ih => -- all
-  have lem := compile_kind_sound_3 wf j2; simp at lem
-  cases lem; case _ A' lem =>
-  cases lem
-  replace ih := @ih (.kind A' :: Γ') (by constructor; assumption; assumption) sorry
-  cases ih; case _ B' ih =>
-  cases ih
-  exists (∀[A']B')
-  constructor;
-  case _ => exists A'; constructor; assumption; exists B'
-  case _ => constructor; assumption; assumption
+-- case _ j1 j2 j3 _ _ ih => -- all
+--   have lem := compile_kind_sound_3 wf j2; simp at lem
+--   cases lem; case _ A' lem =>
+--   cases lem
+--   replace ih := @ih (.kind A' :: Γ') (by constructor; assumption; assumption) sorry
+--   cases ih; case _ B' ih =>
+--   cases ih
+--   exists (∀[A']B')
+--   constructor;
+--   case _ => exists A'; constructor; assumption; exists B'
+--   case _ => constructor; assumption; assumption
 
-case _ Γ _ _ _ _ j1 j2 j3 ih1 _ ih2 => -- app case
-  replace ih2 := @ih2 Γ' wf Γe
-  cases ih2; case _ T' ih2 =>
-  cases ih2; case _ Tk ih2 =>
-  cases ih2; case _ ih2a ih2b =>
-  cases ih2a; case _ κ ih2a =>
-  cases ih2a; case _ ih2a =>
-  cases ih2a; case _ κ' ih2a =>
-  cases ih2a; case _ ih2a =>
-  cases ih2a
-  cases ih2b
+-- case _ Γ _ _ _ _ j1 j2 j3 ih1 _ ih2 => -- app case
+--   replace ih2 := @ih2 Γ' wf Γe
+--   cases ih2; case _ T' ih2 =>
+--   cases ih2; case _ Tk ih2 =>
+--   cases ih2; case _ ih2a ih2b =>
+--   cases ih2a; case _ κ ih2a =>
+--   cases ih2a; case _ ih2a =>
+--   cases ih2a; case _ κ' ih2a =>
+--   cases ih2a; case _ ih2a =>
+--   cases ih2a
+--   cases ih2b
 
-  replace ih1 := @ih1 Γ' wf Γe
-  cases ih1; case _ A' ih1 =>
-  cases ih1; case _ ih1 =>
-  cases ih1; case _ e1 _ _ _ _ e2 ih1 =>
-  rw[e1] at e2; cases e2
-  cases ih1
-  exists (T' `@k A'); exists κ'
-  constructor
-  case _ => assumption
-  case _ =>
-    split
-    case _ T _ _ _ _ _ _ _ _ _ h =>
-      exfalso; simp at h
-      sorry
-    case _ h =>
-      rw[Option.bind_eq_some] at h
-      cases h; case _ h =>
-      cases h; case _ w h1 h2 =>
-      injection h2; case _ h2 =>
-      injection h2; case _ e1 e2 =>
-      split
-      case _ T k k' A _ _ _ _ _ _ _ sp _ tnfp x =>
-        simp
-        have h1' : w = (w.1, w.2) := by simp
-        rw[h1'] at h1
-        rw[Option.bind_eq_some] at h
-        cases h; case _ tnf =>
-        cases tnf; case _ h1a tnf =>
-        rw[h1] at h1a; cases h1a; rw[e1] at h1;
-        have lem := @hs_neutral_form_well_typed .TypeJ (T, k `-k> k') Γ x w.2 j2
-        simp at lem;
-        replace lem := lem h1
-        cases lem; case _ lem1 lem2 =>
-        cases lem1; case _ K lem1 =>
-        constructor;
-        case _ =>
-          have lem3 := Γe x
-          -- Γ s@ x is a tycon or it is a kind
-          cases lem1;
-          case _ lem1 =>
-            rw[lem1] at lem3;
-            replace lem3 := @FrameEquivRefineType Γ Γ' K (Γ' d@ x) lem3
-            cases lem3; case _ K' lem3 =>
-            exists K'
-            constructor
-            case _ => rw[lem3.2]; unfold Frame.get_type; simp; unfold DsM.toDsM; simp
-            case _ =>
-            split
-            case _ =>
-              split
-              case _ => sorry -- well formed kind always splits. contradiction
-              case _ =>
-                split
-                case _ wfk ks ret_k h2 h3 =>
-                  simp at h3; cases h3; case _ h3 h4 =>
-                  cases h3; case _ h3 h5 =>
-                  rw[Option.bind_eq_some] at h2; cases h2; case _ sp' h2 =>
-                  have e := Term.eq_of_beq h3; cases e; clear h3
-                  rw[Except.bind_eq_ok]
+--   replace ih1 := @ih1 Γ' wf Γe
+--   cases ih1; case _ A' ih1 =>
+--   cases ih1; case _ ih1 =>
+--   cases ih1; case _ e1 _ _ _ _ e2 ih1 =>
+--   rw[e1] at e2; cases e2
+--   cases ih1
+--   exists (T' `@k A'); exists κ'
+--   constructor
+--   case _ => assumption
+--   case _ =>
+--     split
+--     case _ T _ _ _ _ _ _ _ _ _ h =>
+--       exfalso; simp at h
+--       sorry
+--     case _ h =>
+--       rw[Option.bind_eq_some_iff] at h
+--       cases h; case _ h =>
+--       cases h; case _ w h1 h2 =>
+--       injection h2; case _ h2 =>
+--       injection h2; case _ e1 e2 =>
+--       split
+--       case _ T k k' A _ _ _ _ _ _ _ sp _ tnfp x =>
+--         simp
+--         have h1' : w = (w.1, w.2) := by simp
+--         rw[h1'] at h1
+--         rw[Option.bind_eq_some_iff] at h
+--         cases h; case _ tnf =>
+--         cases tnf; case _ h1a tnf =>
+--         rw[h1] at h1a; cases h1a; rw[e1] at h1;
+--         have lem := @hs_neutral_form_well_typed .TypeJ (T, k `-k> k') Γ x w.2 j2
+--         simp at lem;
+--         replace lem := lem h1
+--         cases lem; case _ lem1 lem2 =>
+--         cases lem1; case _ K lem1 =>
+--         constructor;
+--         case _ =>
+--           have lem3 := Γe x
+--           -- Γ s@ x is a tycon or it is a kind
+--           cases lem1;
+--           case _ lem1 =>
+--             rw[lem1] at lem3;
+--             replace lem3 := @FrameEquivRefineType Γ Γ' K (Γ' d@ x) lem3
+--             cases lem3; case _ K' lem3 =>
+--             exists K'
+--             constructor
+--             case _ => rw[lem3.2]; unfold Frame.get_type; simp; unfold DsM.toDsM; simp
+--             case _ =>
+--             split
+--             case _ =>
+--               split
+--               case _ => sorry -- well formed kind always splits. contradiction
+--               case _ =>
+--                 split
+--                 case _ wfk ks ret_k h2 h3 =>
+--                   simp at h3; cases h3; case _ h3 h4 =>
+--                   cases h3; case _ h3 h5 =>
+--                   rw[Option.bind_eq_some_iff] at h2; cases h2; case _ sp' h2 =>
+--                   have e := Term.eq_of_beq h3; cases e; clear h3
+--                   rw[Except.bind_eq_ok]
 
-                  sorry
-                case _ => sorry
-            case _ h =>
-            have lem4 : Γ ⊢s `#x : K := by
-              constructor; assumption; apply Or.inr; assumption
-            -- K' is a wf kind contradiction with h
-            exfalso; sorry
-          case _ lem => sorry
+--                   sorry
+--                 case _ => sorry
+--             case _ h =>
+--             have lem4 : Γ ⊢s `#x : K := by
+--               constructor; assumption; apply Or.inr; assumption
+--             -- K' is a wf kind contradiction with h
+--             exfalso; sorry
+--           case _ lem => sorry
 
-        sorry
-      case _ =>
-        split <;> simp at *
-        sorry
-        sorry
+--         sorry
+--       case _ =>
+--         split <;> simp at *
+--         sorry
+--         sorry
