SystemFD/Metatheory/Determined.lean
@@ -1,0 +1,248 @@
+import SystemFD.Term
+import SystemFD.Term.Definition
+import SystemFD.Term.Variant
+import SystemFD.Judgment
+import SystemFD.Ctx
+import SystemFD.Reduction
+import SystemFD.Metatheory.Inversion
+import SystemFD.Metatheory.Weaken
+import SystemFD.Metatheory.Substitution
+import SystemFD.Metatheory.Uniqueness
+import SystemFD.Metatheory.Classification
+import SystemFD.Metatheory.Canonicity
+import SystemFD.Metatheory.Progress
+
+def Term.Determined (Γ : List FrameVariant) (t : Term) : Prop :=
+  ¬ ContainsVariant Γ [.ctor2 .choice, .guard, .zero] t
+
+@[simp]
+def Determined.ctor1 : Term.Determined Γ (.ctor1 v t) <-> Term.Determined Γ t := by
+  apply Iff.intro
+  intro h; apply not_contains_variant_ctor1 h
+  intro h1 h2; cases h2
+  case _ h3 => cases v <;> simp at h3
+  case _ h3 => apply h1 h3
+
+@[simp]
+def Determined.ctor2 :
+  Term.Determined Γ (.ctor2 v t1 t2)
+  <-> v ≠ .choice ∧ Term.Determined Γ t1 ∧ Term.Determined Γ t2
+:= by
+  apply Iff.intro
+  intro h; apply And.intro _; apply not_contains_variant_ctor2 h
+  cases v <;> simp at *; apply h; constructor; simp
+  intro h1 h2; cases h2
+  case _ h3 => cases v <;> simp at h3; apply h1.1 rfl
+  case _ h3 => apply h1.2.1 h3
+  case _ h3 => apply h1.2.2 h3
+
+@[simp]
+def Determined.bind2 :
+  Term.Determined Γ (.bind2 v t1 t2)
+  <-> Term.Determined Γ t1 ∧ Term.Determined (bind2_frame_variant v::Γ) t2
+:= by
+  apply Iff.intro
+  intro h; apply not_contains_variant_bind2 h
+  intro h; rcases h with ⟨h1, h2⟩; intro h3
+  cases h3
+  case _ h3 => cases v <;> simp at h3
+  case _ h3 => apply h1 h3
+  case _ h3 => apply h2 h3
+
+def Determined.beta (f : FrameVariant) :
+  Term.Determined (f::Γ) b ->
+  Term.Determined Γ a ->
+  Term.Determined Γ (b β[a])
+:= by
+  intro h1 h2 h3
+  replace h3 := contains_variant_from_beta f h3
+  cases h3
+  case _ h3 => apply h1 h3
+  case _ h3 => apply h2 h3
+
+inductive Frame.Determined : Frame Term -> Prop
+| openm :
+  Determined (.openm t)
+
+def Determined.openm (Γ : Ctx Term) (i : Nat) : Prop :=
+  ∀ T G sp,
+    Γ d@ i = .openm T ->
+    sp.length ≥ T.arity ->
+    SpineType Γ sp T G ->
+    ∃ t, RedPlus Γ (Term.apply_spine #i sp) t ∧ Term.Determined Γ.variants t
+
+def Determined.letterm (Γ : Ctx Term) (i : Nat) : Prop :=
+  ∀ T t, Γ d@ i = .term T t -> Term.Determined Γ.variants t
+
+def Ctx.Determined (Γ : Ctx Term) : Prop :=
+  ∀ i, Determined.openm Γ i ∧ Determined.letterm Γ i
+
+@[simp]
+abbrev DeterminedProgressLemmaType (Γ : Ctx Term) : (v : JudgmentVariant) -> JudgmentArgs v -> Prop
+| .prf => λ (t, _) =>
+  t.Determined Γ.variants ->
+  Γ.Determined ->
+  Val Γ t ∨ (∃ t', RedPlus Γ t t' ∧ t'.Determined Γ.variants)
+| .wf => λ () => True
+
+theorem determined_progress_lemma :
+  (∀ x, ¬ Γ.is_type x) ->
+  Judgment v Γ ix ->
+  DeterminedProgressLemmaType Γ v ix
+:= by
+  intro h j; induction j <;> simp <;> intros
+  case ax => apply Or.inl; apply Val.star
+  case letterm Γ A t b T j1 j2 j3 j4 ih1 ih2 ih3 ih4 =>
+    sorry
+    -- apply Or.inr; apply Exists.intro (b β[t])
+    -- apply And.intro; apply RedPlus.one Red.letbeta
+    -- cases dt; case _ d1 d2 d3 =>
+    -- sorry
+  case var Γ x T j1 j2 ih dx dΓ =>
+    have j3 := Judgment.var j1 j2
+    replace h := h x
+    generalize fdef : Γ d@ x = f at *
+    cases f <;> simp [Frame.get_type] at *
+    all_goals rw [fdef] at h; simp [Frame.is_type] at h
+    all_goals subst j2; clear ih h
+    case openm =>
+      cases Nat.decLt 0 T.arity
+      case _ h =>
+        generalize zdef : T.to_telescope = z
+        rcases z with ⟨γ, G⟩; simp at h
+        have lem0 := inversion_apply_spine (sp := []) j3
+        rcases lem0 with ⟨C, q1, q2, q3⟩
+        cases q2; case _ c q2 =>
+        clear c; rw [fdef] at q2; simp [Frame.get_type] at q2; subst q2
+        replace dΓ := (dΓ x).1 C C [] fdef (by simp; exact h) q1
+        rcases dΓ with ⟨t, r, dt⟩
+        apply Or.inr; apply Exists.intro t
+        apply And.intro r dt
+      case _ h =>
+        apply Or.inl; apply Val.app (x := x) (sp := []); simp
+        apply Or.inr; simp [OpenVarVal]; rw [fdef]; simp [Frame.is_openm]
+        intro S sh; simp [Frame.get_type] at sh; subst sh
+        apply h
+    case term t =>
+      have lem := (dΓ x).2 T t fdef
+      apply Or.inr; apply Exists.intro t
+      apply And.intro _ lem
+      apply RedPlus.one
+      have r := @Red.letterm #x x [] Γ T t; simp at r
+      apply r; rw [fdef]
+    all_goals
+      apply Or.inl; apply Val.app x []; simp
+      apply Or.inl; simp; rw [fdef]; simp [Frame.is_stable_red]
+  case allk => apply Or.inl; apply Val.arrk
+  case allt => apply Or.inl; apply Val.all
+  case arrow => apply Or.inl; apply Val.arr
+  case appk Γ f A B a j1 j2 ih1 ih2 df da dΓ =>
+    have lem1 := classification_lemma j1; simp at lem1
+    rcases lem1 with ⟨lem1⟩ | ⟨K, j3, j4⟩; rotate_left
+    cases j4; cases j3; cases lem1; case _ j3 j4 =>
+    have j5 := Judgment.appk j1 j2
+    apply Or.inl; apply types_are_values j5 j4
+  case eq => apply Or.inl; apply Val.eq
+  case ite => sorry
+  case guard dt _ => exfalso; apply dt; constructor; simp
+  case lam => apply Or.inl; apply Val.lam
+  case app Γ f A B a B' j1 j2 j3 ih1 ih2 df da dΓ =>
+    simp at ih1 h; replace ih1 := ih1 h df dΓ
+    rcases ih1 with ⟨ih1⟩ | ⟨f', r, ih1⟩; rotate_left
+    apply Or.inr; apply Exists.intro (f' `@ a)
+    apply And.intro; apply RedPlus.ctor2_congr1 rfl r
+    apply Determined.ctor2.2; simp; apply And.intro ih1 da
+    cases ih1
+    case app x sp h1 h2 =>
+      cases h1
+      case _ h1 =>
+        apply Or.inl; apply Val.app x (sp ++ [(.term, a)]) _ (Or.inl h1)
+        simp; rw [Option.bind_eq_some_iff]
+        apply Exists.intro (x, sp); simp [*]
+      case _ h1 =>
+        simp [OpenVarVal] at h1
+        generalize fdef : Γ d@x = f at *
+        cases f <;> simp [Frame.is_openm] at h1; case _ T =>
+        cases Nat.decLt (sp ++ [(SpineVariant.term, a)]).length T.arity
+        case _ h3 =>
+          simp at h3; apply Or.inr
+          replace h2 := Term.neutral_form_law (Eq.symm h2); subst h2
+          have j4 := Judgment.app j1 j2 j3; rw [<-Term.apply_spine_peel_term] at *
+          have lem1 := inversion_apply_spine j4
+          rcases lem1 with ⟨C, lem1, lem2, lem3⟩
+          cases lem2; case _ j5 j6 =>
+          rw [fdef] at j6; simp [Frame.get_type] at j6; subst j6
+          replace h1 := h1 C (by simp [Frame.get_type])
+          replace h1 : C.arity = sp.length + 1 := by omega
+          replace dΓ := (dΓ x).1 C B' (sp ++ [(SpineVariant.term, a)]) fdef (by simp; omega) lem1
+          rcases dΓ with ⟨t, r, dt⟩
+          apply Exists.intro t; apply And.intro r dt
+        case _ h3 =>
+          simp at h3; apply Or.inl; apply Val.app x (sp ++ [(.term, a)])
+          simp; rw [Option.bind_eq_some_iff]
+          apply Exists.intro (x, sp); simp [*]
+          apply Or.inr; simp [OpenVarVal]; rw [fdef]; simp [Frame.is_openm]
+          intro S sh; simp [Frame.get_type] at sh; subst sh
+          apply h3
+    case choice => simp at df
+    case lam C b =>
+      apply Or.inr; apply Exists.intro (b β[a])
+      apply And.intro; apply RedPlus.one Red.beta
+      simp at df; apply Determined.beta _ df.2 da
+    all_goals (cases j1)
+  case lamt => apply Or.inl; apply Val.lamt
+  case appt Γ f A B a B' j1 j2 j3 ih1 ih2 df da dΓ =>
+    simp at ih1 h; replace ih1 := ih1 h df dΓ
+    rcases ih1 with ⟨ih1⟩ | ⟨f', r, ih1⟩; rotate_left
+    apply Or.inr; apply Exists.intro (f' `@t a)
+    apply And.intro; apply RedPlus.ctor2_congr1 rfl r
+    apply Determined.ctor2.2; simp; apply And.intro ih1 da
+    cases ih1
+    case app x sp h1 h2 =>
+      cases h1
+      case _ h1 =>
+        apply Or.inl; apply Val.app x (sp ++ [(.type, a)]) _ (Or.inl h1)
+        simp; rw [Option.bind_eq_some_iff]
+        apply Exists.intro (x, sp); simp [*]
+      case _ h1 =>
+        simp [OpenVarVal] at h1
+        generalize fdef : Γ d@x = f at *
+        cases f <;> simp [Frame.is_openm] at h1; case _ T =>
+        cases Nat.decLt (sp ++ [(SpineVariant.type, a)]).length T.arity
+        case _ h3 =>
+          simp at h3; apply Or.inr
+          replace h2 := Term.neutral_form_law (Eq.symm h2); subst h2
+          have j4 := Judgment.appt j1 j2 j3; rw [<-Term.apply_spine_peel_type] at *
+          have lem1 := inversion_apply_spine j4
+          rcases lem1 with ⟨C, lem1, lem2, lem3⟩
+          cases lem2; case _ j5 j6 =>
+          rw [fdef] at j6; simp [Frame.get_type] at j6; subst j6
+          replace h1 := h1 C (by simp [Frame.get_type])
+          replace h1 : C.arity = sp.length + 1 := by omega
+          replace dΓ := (dΓ x).1 C B' (sp ++ [(SpineVariant.type, a)]) fdef (by simp; omega) lem1
+          rcases dΓ with ⟨t, r, dt⟩
+          apply Exists.intro t; apply And.intro r dt
+        case _ h3 =>
+          simp at h3; apply Or.inl; apply Val.app x (sp ++ [(.type, a)])
+          simp; rw [Option.bind_eq_some_iff]
+          apply Exists.intro (x, sp); simp [*]
+          apply Or.inr; simp [OpenVarVal]; rw [fdef]; simp [Frame.is_openm]
+          intro S sh; simp [Frame.get_type] at sh; subst sh
+          apply h3
+    case choice => simp at df
+    case lamt C b =>
+      apply Or.inr; apply Exists.intro (b β[a])
+      apply And.intro; apply RedPlus.one Red.betat
+      simp at df; apply Determined.beta _ df.2 da
+    all_goals (cases j1)
+  case cast => sorry
+  case refl => sorry
+  case sym => sorry
+  case seq => sorry
+  case appc => sorry
+  case arrowc => sorry
+  case fst => sorry
+  case snd => sorry
+  case allc => sorry
+  case apptc => sorry
+  case empty dt _ => exfalso; apply dt; constructor; simp
