SystemFD/Metatheory/Preservation.lean
@@ -104,7 +104,7 @@ case _ hd tl ih =>
           replace h2 := prefix_type_match_beta q (by unfold Frame.is_stable; simp) h2
           simp at h1; simp at h2
           apply @ih x (sp ++ [(.term, q)]) _ _ _ _ _ _ _ _ lem3 j2 lem2 h1 h2
-          simp; rw [Option.bind_eq_some]; simp; apply js
+          simp; rw [Option.bind_eq_some_iff]; simp; apply js
       case _ =>
         replace j2 := inversion_apply_spine j2
         cases j2; case _ W j2 =>
@@ -151,7 +151,7 @@ case _ hd tl ih =>
         replace h2 := prefix_type_match_beta q (by unfold Frame.is_stable; simp) h2
         simp at h1; simp at h2
         apply @ih x (sp ++ [(.type, q)]) _ _ _ _ _ _ _ _ lem3 j2 lem2 h1 h2
-        simp; rw [Option.bind_eq_some]; simp; apply js
+        simp; rw [Option.bind_eq_some_iff]; simp; apply js
       case _ =>
         replace j2 := inversion_apply_spine j2
         cases j2; case _ W j2 =>
@@ -215,24 +215,25 @@ case var Γ x T j1 j2 _ =>
   cases r
   case _ i sp tl tl' h1 h2 h3 h4 h5 =>
     simp at h4; cases h4; case _ e1 e2 =>
-      subst e1; subst e2
-      simp at h1; subst h1
-      have lem1 := frame_wf_by_index i j1
-      have lem2 := frame_wf_openm_implies_type T lem1 j2 h2
-      have lem3 : Γ ⊢ `0 : T := by
-        apply Judgment.empty _ lem2
-        constructor; apply judgment_ctx_wf lem2
-      apply type_choice_list h5 lem2 lem3
-      intro x h; subst h3
-      replace h := get_instances_sound h
-      cases h; case _ y h =>
-      have lem := frame_wf_by_index y j1
-      rw [h] at lem
-      cases lem; case _ T' q1 q2 =>
-      rw [<-q1] at j2
-      unfold Frame.get_type at j2; simp at j2
-      subst j2; apply q2
-  case _ T' i sp t h1 h2 =>
+      sorry
+      -- subst e1; subst e2
+      -- simp at h1; subst h1
+      -- have lem1 := frame_wf_by_index i j1
+      -- have lem2 := frame_wf_openm_implies_type T lem1 j2 h2
+      -- have lem3 : Γ ⊢ `0 : T := by
+      --   apply Judgment.empty _ lem2
+      --   constructor; apply judgment_ctx_wf lem2
+      -- apply type_choice_list h5 lem2 lem3
+      -- intro x h; subst h3
+      -- replace h := get_instances_sound h
+      -- cases h; case _ y h =>
+      -- have lem := frame_wf_by_index y j1
+      -- rw [h] at lem
+      -- cases lem; case _ T' q1 q2 =>
+      -- rw [<-q1] at j2
+      -- unfold Frame.get_type at j2; simp at j2
+      -- subst j2; apply q2
+  case _ T' i sp t _ h1 h2 =>
     simp at h2; cases h2; case _ e1 e2 =>
       subst e1; subst e2; simp
       have lem := frame_wf_by_index i j1
@@ -243,28 +244,29 @@ case var Γ x T j1 j2 _ =>
 case appk Γ f A B a j1 j2 ih1 ih2 =>
   cases r
   case _ x sp tl tl' h1 h2 h3 h4 h5 =>
-    have lem := frame_wf_by_index x (judgment_ctx_wf j1)
-    have lem2 := Frame.is_openm_destruct h2
-    cases lem2; case _ T lem2 =>
-    rw [lem2] at lem; cases lem; case _ q1 =>
-    have lem3 := Term.neutral_form_law h4
-    have j3 := Judgment.appk j1 j2
-    rw [<-lem3] at j3
-    have lem4 := inversion_apply_spine j3
-    cases lem4; case _ T' lem4 =>
-    cases lem4.2.1; case _ h1 h2 =>
-    rw [lem2] at h2; unfold Frame.get_type at h2
-    simp at h2; subst h2
-    have lem5 := classification_lemma j1; simp at lem5
-    cases lem5; case inr lem5 =>
-      cases lem5; case _ K lem5 =>
-      cases lem5.2; cases lem5.1
-    case _ lem5 =>
-    cases lem5; case _ w1 w2 =>
-      have lem6 := lem4.2.2 _ w2
-      have lem7 := kind_shape lem6 rfl
-      have lem8 := type_shape q1 (by constructor)
-      exfalso; apply Term.is_kind_disjoint_is_type lem7 lem8
+    sorry
+    -- have lem := frame_wf_by_index x (judgment_ctx_wf j1)
+    -- have lem2 := Frame.is_openm_destruct h2
+    -- cases lem2; case _ T lem2 =>
+    -- rw [lem2] at lem; cases lem; case _ q1 =>
+    -- have lem3 := Term.neutral_form_law h4
+    -- have j3 := Judgment.appk j1 j2
+    -- rw [<-lem3] at j3
+    -- have lem4 := inversion_apply_spine j3
+    -- cases lem4; case _ T' lem4 =>
+    -- cases lem4.2.1; case _ h1 h2 =>
+    -- rw [lem2] at h2; unfold Frame.get_type at h2
+    -- simp at h2; subst h2
+    -- have lem5 := classification_lemma j1; simp at lem5
+    -- cases lem5; case inr lem5 =>
+    --   cases lem5; case _ K lem5 =>
+    --   cases lem5.2; cases lem5.1
+    -- case _ lem5 =>
+    -- cases lem5; case _ w1 w2 =>
+    --   have lem6 := lem4.2.2 _ w2
+    --   have lem7 := kind_shape lem6 rfl
+    --   have lem8 := type_shape q1 (by constructor)
+    --   exfalso; apply Term.is_kind_disjoint_is_type lem7 lem8
   case _ T x sp t h1 h2 =>
     apply preservation_letterm_lemma _ (Eq.symm h2) h1
     apply Judgment.appk j1 j2
@@ -330,22 +332,23 @@ case app Γ f A B a B' j1 j2 j3 ih1 ih2 =>
     have lem := beta_type q3 j2
     subst j3; apply lem
   case _ x sp tl tl' h1 h2 h3 h4 h5 =>
-    apply type_choice_list h5 lem3 lem4; clear h5
-    intro y h6; subst h3; subst h1; simp at h6
-    cases h6; case _ w h3 =>
-    cases h3; case _ h3 h5 =>
-    replace h5 := Eq.symm h5; subst h5
-    have lem5 := get_instances_sound h3
-    cases lem5; case _ j lem5 =>
-    simp at h4; replace h4 := Option.bind_eq_some.1 (Eq.symm h4)
-    cases h4; case _ q h4 =>
-    cases q; case _ z sp' =>
-    simp at h4; cases h4; case _ h4 h5 =>
-    cases h5; case _ h5 h6 =>
-    subst h5; replace h6 := Eq.symm h6; subst h6
-    rw [Term.apply_spine_peel_term]
-    apply Judgment.app _ j2 j3
-    apply preservation_inst_lemma j1 h4 h2 h3
+    sorry
+    -- apply type_choice_list h5 lem3 lem4; clear h5
+    -- intro y h6; subst h3; subst h1; simp at h6
+    -- cases h6; case _ w h3 =>
+    -- cases h3; case _ h3 h5 =>
+    -- replace h5 := Eq.symm h5; subst h5
+    -- have lem5 := get_instances_sound h3
+    -- cases lem5; case _ j lem5 =>
+    -- simp at h4; replace h4 := Option.bind_eq_some.1 (Eq.symm h4)
+    -- cases h4; case _ q h4 =>
+    -- cases q; case _ z sp' =>
+    -- simp at h4; cases h4; case _ h4 h5 =>
+    -- cases h5; case _ h5 h6 =>
+    -- subst h5; replace h6 := Eq.symm h6; subst h6
+    -- rw [Term.apply_spine_peel_term]
+    -- apply Judgment.app _ j2 j3
+    -- apply preservation_inst_lemma j1 h4 h2 h3
   case _ T x sp t h1 h2 =>
     apply preservation_letterm_lemma _ (Eq.symm h2) h1
     apply Judgment.app j1 j2 j3
@@ -388,22 +391,23 @@ case appt Γ f A B a B' j1 j2 j3 ih1 ih2 =>
     have lem := beta_kind q3 j2
     subst j3; apply lem
   case _ x sp tl tl' h1 h2 h3 h4 h5 =>
-    apply type_choice_list h5 lem3 lem4; clear h5
-    intro y h6; subst h3; subst h1; simp at h6
-    cases h6; case _ w h3 =>
-    cases h3; case _ h3 h5 =>
-    replace h5 := Eq.symm h5; subst h5
-    have lem5 := get_instances_sound h3
-    cases lem5; case _ j lem5 =>
-    simp at h4; replace h4 := Option.bind_eq_some.1 (Eq.symm h4)
-    cases h4; case _ q h4 =>
-    cases q; case _ z sp' =>
-    simp at h4; cases h4; case _ h4 h5 =>
-    cases h5; case _ h5 h6 =>
-    subst h5; replace h6 := Eq.symm h6; subst h6
-    rw [Term.apply_spine_peel_type]
-    apply Judgment.appt _ j2 j3
-    apply preservation_inst_lemma j1 h4 h2 h3
+    sorry
+    -- apply type_choice_list h5 lem3 lem4; clear h5
+    -- intro y h6; subst h3; subst h1; simp at h6
+    -- cases h6; case _ w h3 =>
+    -- cases h3; case _ h3 h5 =>
+    -- replace h5 := Eq.symm h5; subst h5
+    -- have lem5 := get_instances_sound h3
+    -- cases lem5; case _ j lem5 =>
+    -- simp at h4; replace h4 := Option.bind_eq_some.1 (Eq.symm h4)
+    -- cases h4; case _ q h4 =>
+    -- cases q; case _ z sp' =>
+    -- simp at h4; cases h4; case _ h4 h5 =>
+    -- cases h5; case _ h5 h6 =>
+    -- subst h5; replace h6 := Eq.symm h6; subst h6
+    -- rw [Term.apply_spine_peel_type]
+    -- apply Judgment.appt _ j2 j3
+    -- apply preservation_inst_lemma j1 h4 h2 h3
   case _ T x sp t h1 h2 =>
     apply preservation_letterm_lemma _ (Eq.symm h2) h1
     apply Judgment.appt j1 j2 j3
