SystemFD/Util.lean
@@ -32,7 +32,7 @@ cases t; simp
 case _ v => exfalso; apply h v rfl
 
 theorem not_eq_of_beq [BEq T] [LawfulBEq T] {x y : T} : ¬ ((x == y) = true) -> x ≠ y := by
-intro h1 h2; subst h2; apply h1; apply LawfulBEq.rfl
+intro h1 h2; subst h2; apply h1; simp
 
 @[simp]
 def rep (f : T -> T) (x : T) : Nat -> T
